Test/uncooperativeconcurrency/concurrentarray.dfy
@@ -1,0 +1,78 @@
+
+
+// Concurrent array that resizes on demand.
+// Essentially like a caching map from nat -> T
+class {:separated} ConcurrentArray<T> {
+
+    ghost const inv: T -> bool
+
+    // TODO: This may need to be more like an Action<(), T> to
+    // create the value if T is a reference type.
+    // But it might be better to just use T? with null in that case instead.
+    const default: T
+    var storage: array<T>
+
+    ghost var {:separatedHeap} Repr: set<object>
+
+    ghost predicate Valid() 
+      reads this, Repr
+    {
+      && this in Repr
+      && storage in Repr
+      && inv(default)
+      && forall t <- storage[..] :: inv(t)
+      // && forall v <- Items :: v.Owner == this
+    }
+
+    constructor(default: T, ghost inv: T -> bool) 
+      requires inv(default)
+    {
+      this.default := default;
+      this.storage := new T[10](i => default);
+    }
+
+    function Select(i: nat): (r: T)
+      requires Valid()
+      reads this, Repr
+      ensures inv(r)
+    {
+      if i < storage.Length then
+        storage[i]
+      else
+        default
+    }
+
+    method Update(i: nat, newValue: T) 
+      requires Valid()
+      modifies Repr
+    {
+      if storage.Length <= i {
+        Resize(i + 1);
+      }
+      assert i < storage.Length;
+      storage[i] := newValue;
+    }
+
+    method Resize(newCapacity: int)
+      requires Valid()
+      // TODO: accidentally got away with not writing Repr here,
+      // but Valid() ==> this in Repr, so that should be legal still?
+      modifies this
+      ensures Valid()
+      ensures fresh(Repr - old(Repr))
+      ensures old(storage.Length) <= storage.Length
+      ensures newCapacity <= storage.Length
+    {
+      if newCapacity <= storage.Length {
+        return;
+      }
+      var newStorage := new T[newCapacity](i => default);
+      // Ideally this could be compiled to an optimized array copy
+      // (e.g. System.arraycopy in Java)
+      forall i | 0 <= i < storage.Length {
+        newStorage[i] := storage[i];
+      }
+      storage := newStorage;
+      Repr := {this, storage};
+    }
+  }
