Test/uncooperativeconcurrency/concurrentlinkedlist.dfy
@@ -1,0 +1,245 @@
+
+include "separatedclass.dfy"
+
+// Modified version of this datatype:
+// https://github.com/aws/aws-cryptographic-material-providers-library-java/blob/main/AwsCryptographicMaterialProviders/dafny/AwsCryptographicMaterialProviders/src/CMCs/LocalCMC.dfy#L65
+module ConcurrentDoublyLinkedList {
+
+  import opened SeparatedClasses
+
+  datatype Ref<T> =
+    | Ptr(deref: T)
+    | Null
+
+
+  class ConcurrentDoublyLinkedList<T> extends OwnedObject {
+
+    // New for the concurrent version
+    ghost const inv: T -> bool
+    
+    var head: Ref<LinkedListNode<T>>
+    var tail: Ref<LinkedListNode<T>>
+
+    ghost var Items: seq<LinkedListNode<T>>
+
+    constructor(ghost inv: T -> bool)
+      ensures Invariant()
+      ensures this.inv == inv
+    {
+      // Forced by being a separated class
+      Owner := this;
+
+      this.inv := inv;
+      head := Null;
+      tail := Null;
+      Items := [];
+    }
+
+    ghost predicate Invariant()
+      reads this, Items
+    {
+      // head and tail properties
+      && (0 == |Items| <==> head.Null? && tail.Null?)
+      && (0 < |Items| <==>
+          && head.Ptr?
+          && tail.Ptr?
+          && head.deref == Items[0]
+          && tail.deref == Items[|Items| - 1])
+      && (head.Ptr? <==> tail.Ptr?)
+      && (head.Ptr? ==> head.deref.prev.Null?)
+      && (tail.Ptr? ==> tail.deref.next.Null?)
+          // Every Cell in the DoublyLinkedList MUST be unique.
+          // Otherwise there would be loops in prev and next.
+          // For a Cell at 4, next MUST point to 5 or Null?.
+          // So if a Cell exists as 4 and 7
+          // then it's next would need to point to _both_ 5 and 8.
+      && (forall v <- Items :: multiset(Items)[v] == 1)
+          // Proving order is easier by being more specific
+          // and breaking up prev and next.
+          // Order means Cell 4 point to 3 and 5
+          // in prev and next respectively.
+      && (forall i: nat | 0 <= i < |Items| ::
+            && Prev?(i, Items[i], Items)
+            && Next?(i, Items[i], Items)
+          )
+      // New for the concurrent version
+      && forall v <- Items :: inv(v.value)
+      && forall v <- Items :: v.Owner == this
+    }
+
+    ghost predicate Prev?(i:nat, c: LinkedListNode<T>, Items' : seq<LinkedListNode<T>>)
+      reads Items'
+      requires 0 <= i < |Items'|
+      requires Items'[i] == c
+    {
+      if i == 0 then
+        Items'[0].prev.Null?
+      else
+        && Items'[i].prev.Ptr?
+        && Items'[i].prev.deref == Items'[i - 1]
+    }
+
+    ghost predicate Next?(i:nat, c: LinkedListNode<T>, Items' : seq<LinkedListNode<T>>)
+      reads Items'
+      requires 0 <= i < |Items'|
+      requires Items'[i] == c
+    {
+      if i < |Items'| -1 then
+        && Items'[i].next.Ptr?
+        && Items'[i].next.deref == Items'[i + 1]
+      else
+        assert i == |Items'| - 1;
+        && Items'[i].next.Null?
+    }
+
+    method PushCell(toPush: LinkedListNode<T>)
+      requires toPush !in Items
+      requires toPush.next.Null? && toPush.prev.Null?
+      // New for concurrent version
+      requires toPush.Owner == this;
+      requires Invariant()
+      requires inv(toPush.value)
+      modifies this, Items, toPush
+      ensures Invariant()
+    {
+      Items := [toPush] + Items;
+
+      var cRef := Ptr(toPush);
+      if head.Ptr? {
+        assert head.deref in Items;
+        assert CanAccess(head.deref);
+        head.deref.prev := cRef;
+        toPush.next := head;
+        head := cRef;
+      } else {
+        assert CanAccess(this);
+        head := cRef;
+        tail := head;
+      }
+    }
+
+    method Push(value: T)
+      requires Invariant()
+      requires inv(value)
+      modifies this, Items
+      ensures Invariant()
+    {
+      var toPush := new LinkedListNode<T>(value);
+      toPush.Owner := this;
+      PushCell(toPush);
+    }
+
+    method {:vcs_split_on_every_assert} Remove(toRemove: LinkedListNode<T>)
+      requires Invariant()
+      requires toRemove in Items
+      modifies this, Items
+      ensures Invariant()
+      ensures multiset(Items) == multiset(old(Items)) - multiset{toRemove}
+      ensures toRemove !in Items
+      ensures toRemove.next.Null? && toRemove.prev.Null?
+      ensures toRemove.Owner == null
+      ensures |Items| < |old(Items)|
+    {
+      ghost var pos := IndexOfNode(Items, toRemove);
+      // This is s[..pos] + s[pos+1]
+      // where pos :| s[pos] == c
+      Items := RemoveNode(Items, toRemove);
+
+      if toRemove.prev.Null? {
+        // toRemove is head
+        assert toRemove.prev.Null? ==> Ptr(toRemove) == head;
+        assert pos == 0;
+        head := toRemove.next;
+      } else {
+        // toRemove is !head
+        assert toRemove != head.deref;
+        assert 0 != pos;
+        assert 0 < |Items|;
+        assert Items[pos - 1] == toRemove.prev.deref;
+        toRemove.prev.deref.next := toRemove.next;
+      }
+
+      if toRemove.next.Null? {
+        // toRemove is tail
+        assert toRemove.next.Null? ==> Ptr(toRemove) == tail;
+        tail := toRemove.prev;
+      } else {
+        // toRemove is !tail
+        assert toRemove != tail.deref;
+        assert 0 < |Items|;
+        toRemove.next.deref.prev := toRemove.prev;
+      }
+
+      label AFTER:
+
+      assert {:split_here} true;
+      assert Items == old@AFTER(Items);
+      assert toRemove !in Items;
+
+      toRemove.next := Null;
+      toRemove.prev := Null;
+      SetOwner(toRemove, null);
+    }
+
+    // TODO: seems like it should be a general Seq utility...
+    ghost function {:opaque} RemoveNode(s: seq<LinkedListNode<T>>, v: LinkedListNode<T>): (s': seq<LinkedListNode<T>>)
+      requires multiset(s)[v] == 1
+      ensures v !in s'
+      ensures multiset(s') == multiset(s) - multiset{v}
+      ensures
+        var pos := IndexOfNode(s, v);
+        && (forall i: nat | 0 <= i < pos :: s[i] == s'[i])
+        && (forall i: nat | pos <= i < |s'| :: s[i+1] == s'[i])
+        && (s' == s[..pos] + s[pos+1..])
+    {
+      var pos := IndexOfNode(s, v);
+      // Associativity, s[pos..] is the sum of both sides
+      assert s == s[..pos] + s[pos..];
+      // the 1 v MUST be in the right side
+      assert multiset(s[pos..])[v] == 1;
+      // Associativity, s[pos..] is the sum of both sides
+      assert s[pos..] == [s[pos]] + s[pos+1..];
+      s[..pos] + s[pos+1..]
+    }
+
+    ghost function IndexOfNode(s: seq<LinkedListNode<T>>, v: LinkedListNode<T>): (pos: nat)
+      requires v in s
+      ensures pos < |s| && s[pos] == v
+      ensures v !in s[..pos]
+    {
+      if s[0] == v then 0 else 1 + IndexOfNode(s[1..], v)
+    }
+
+    // New for concurrent version
+    method SplitBy(p: T -> bool) returns (matching: ConcurrentDoublyLinkedList<T>) 
+      ensures Invariant()
+      ensures matching.Invariant()
+      ensures multiset(old(Items)) == multiset(Items) + multiset(matching.Items)
+      ensures multiset(Items) !! multiset(matching.Items)
+      ensures forall i | 0 <= i < |Items| :: !p(Items[i].value)
+      ensures forall i | 0 <= i < |matching.Items| :: p(matching.Items[i].value)
+      // TODO: Something about order too
+
+    method FindBy(p: T -> bool) returns (result: LinkedListNode?<T>) 
+      ensures result != null <==> exists item <- Items :: p(item.value)
+      // TODO: Something about order too
+   }
+
+  class LinkedListNode<T> extends OwnedObject {
+    var value: T
+    var next: Ref<LinkedListNode<T>>
+    var prev: Ref<LinkedListNode<T>>
+
+    constructor(value: T) 
+      ensures this.value == value
+      ensures next == Null
+      ensures prev == Null
+    {
+      this.value := value;
+      next := Null;
+      prev := Null;
+    }
+  }
+
+}
+
